SafeAccess.v
@@ -8,56 +8,6 @@ From Elo Require Import Core.
 From Elo Require Import Access.
 From Elo Require Import References.
 
-(* ------------------------------------------------------------------------- *)
-(* SafeAccess & UnsafeAccess                                                 *)
-(* ------------------------------------------------------------------------- *)
-
-Inductive UnsafeAccess (m : mem) : tm -> addr -> Prop :=
-  | uacc_mem : forall ad ad' T,
-    ad <> ad' ->
-    UnsafeAccess m m[ad'] ad ->
-    UnsafeAccess m <{ &ad' :: T }> ad
-
-  | uacc_ref : forall ad T,
-    UnsafeAccess m <{ &ad :: &T }> ad
-
-  | uacc_new : forall T t ad,
-    UnsafeAccess m t ad ->
-    UnsafeAccess m <{ new T t }> ad
-
-  | uacc_load : forall t ad,
-    UnsafeAccess m t ad ->
-    UnsafeAccess m <{ *t }> ad
-
-  | uacc_asg1 : forall t1 t2 ad,
-    UnsafeAccess m t1 ad ->
-    UnsafeAccess m <{ t1 = t2 }> ad
-
-  | uacc_asg2 : forall t1 t2 ad,
-    UnsafeAccess m t2 ad ->
-    UnsafeAccess m <{ t1 = t2 }> ad
-
-  | uacc_fun : forall x Tx t ad,
-    UnsafeAccess m t ad ->
-    UnsafeAccess m <{ fn x Tx --> t }> ad
-
-  | uacc_call1 : forall t1 t2 ad,
-    UnsafeAccess m t1 ad ->
-    UnsafeAccess m <{ call t1 t2 }> ad
-
-  | uacc_call2 : forall t1 t2 ad,
-    UnsafeAccess m t2 ad ->
-    UnsafeAccess m <{ call t1 t2 }> ad
-
-  | uacc_seq1 : forall t1 t2 ad,
-    UnsafeAccess m t1 ad ->
-    UnsafeAccess m <{ t1; t2 }> ad
-
-  | uacc_seq2 : forall t1 t2 ad,
-    UnsafeAccess m t2 ad ->
-    UnsafeAccess m <{ t1; t2 }> ad
-  .
-
 Inductive SafeAccess (m : mem) : tm -> addr -> Prop :=
   | sacc_mem : forall ad ad' T,
     ad <> ad' ->
@@ -82,12 +32,12 @@ Inductive SafeAccess (m : mem) : tm -> addr -> Prop :=
 
   | sacc_asg1 : forall t1 t2 ad,
     SafeAccess m t1 ad ->
-    ~ UnsafeAccess m t2 ad ->
+    ~ access m t2 ad ->
     SafeAccess m <{ t1 = t2 }> ad
 
   | sacc_asg2 : forall t1 t2 ad,
     SafeAccess m t2 ad ->
-    ~ UnsafeAccess m t1 ad ->
+    ~ access m t1 ad ->
     SafeAccess m <{ t1 = t2 }> ad
 
   | sacc_fun : forall x Tx t ad,
@@ -101,15 +51,14 @@ Inductive SafeAccess (m : mem) : tm -> addr -> Prop :=
 
   | sacc_call1 : forall t1 t2 ad,
     SafeAccess m t1 ad ->
-    ~ UnsafeAccess m t2 ad ->
+    ~ access m t2 ad ->
     SafeAccess m <{ call t1 t2 }> ad
 
   | sacc_call2 : forall t1 t2 ad,
     SafeAccess m t2 ad ->
-    ~ UnsafeAccess m t1 ad ->
+    ~ access m t1 ad ->
     SafeAccess m <{ call t1 t2 }> ad
 
-  (* TODO: redundante *)
   | sacc_seq : forall t1 t2 ad,
     SafeAccess m t1 ad ->
     SafeAccess m t2 ad ->
@@ -117,12 +66,12 @@ Inductive SafeAccess (m : mem) : tm -> addr -> Prop :=
 
   | sacc_seq1 : forall t1 t2 ad,
     SafeAccess m t1 ad ->
-    ~ UnsafeAccess m t2 ad ->
+    ~ access m t2 ad ->
     SafeAccess m <{ t1; t2 }> ad
 
   | sacc_seq2 : forall t1 t2 ad,
     SafeAccess m t2 ad ->
-    ~ UnsafeAccess m t1 ad ->
+    ~ access m t1 ad ->
     SafeAccess m <{ t1; t2 }> ad
   .
 
@@ -141,109 +90,28 @@ Ltac inversion_sacc :=
   | H : SafeAccess _ <{ spawn _      }> _ |- _ => inversion_subst_clear H
   end.
 
-Ltac inversion_uacc :=
-  match goal with
-  | H : UnsafeAccess _ <{ unit         }> _ |- _ => inversion_subst_clear H
-  | H : UnsafeAccess _ <{ N _          }> _ |- _ => inversion_subst_clear H
-  | H : UnsafeAccess _ <{ & _ :: _     }> _ |- _ => inversion_subst_clear H
-  | H : UnsafeAccess _ <{ new _ _      }> _ |- _ => inversion_subst_clear H
-  | H : UnsafeAccess _ <{ * _          }> _ |- _ => inversion_subst_clear H
-  | H : UnsafeAccess _ <{ _ = _        }> _ |- _ => inversion_subst_clear H
-  | H : UnsafeAccess _ <{ var _        }> _ |- _ => inversion_subst_clear H
-  | H : UnsafeAccess _ <{ fn _ _ --> _ }> _ |- _ => inversion_subst_clear H
-  | H : UnsafeAccess _ <{ call _ _     }> _ |- _ => inversion_subst_clear H
-  | H : UnsafeAccess _ <{ _ ; _        }> _ |- _ => inversion_subst_clear H
-  | H : UnsafeAccess _ <{ spawn _      }> _ |- _ => inversion_subst_clear H
-  end.
-
-(* ------------------------------------------------------------------------- *)
-(* Properties                                                                *)
-(* ------------------------------------------------------------------------- *)
-
-Theorem sacc_then_access : forall m t ad,
+Lemma sacc_then_access : forall m t ad,
   SafeAccess m t ad ->
   access m t ad.
 Proof.
   intros * H. induction H; eauto using access.
 Qed.
 
-Theorem uacc_then_access : forall m t ad,
-  UnsafeAccess m t ad ->
-  access m t ad.
+Lemma not_access_then_not_sacc : forall m t ad,
+  ~ access m t ad ->
+  ~ SafeAccess m t ad.
 Proof.
-  intros * H. induction H; eauto using access.
+  intros * H F. induction F; eauto using access.
 Qed.
 
-Theorem not_uacc_sacc : forall m t ad,
-  UnsafeAccess m t ad ->
-  SafeAccess m t ad ->
-  False.
-Proof.
-  intros * Huacc ?. induction Huacc; inversion_sacc; eauto.
-Qed.
+(*
 
-Theorem access_to_uacc : forall Gamma m t ad T,
-  Gamma |-- t is T ->
-  well_typed_memory m ->
-  access m t ad ->
-  ~ SafeAccess m t ad ->
-  UnsafeAccess m t ad.
-Proof.
-  intros * ? Hwtm Hacc ?.
-  generalize dependent Gamma. generalize dependent T.
-  induction Hacc; intros; inversion_type; eauto using UnsafeAccess;
-  unshelve solve 
-    [ exfalso; eauto using SafeAccess
-    | assert (~ SafeAccess m t ad) by shelve; eauto using UnsafeAccess
-    | assert (H1' : ~ (SafeAccess m t1 ad /\ SafeAccess m t2 ad)) by shelve;
-      assert (H2' : ~ (SafeAccess m t1 ad /\ ~ UnsafeAccess m t2 ad)) by shelve;
-      assert (H3' : ~ (SafeAccess m t2 ad /\ ~ UnsafeAccess m t1 ad)) by shelve;
-      eapply not_and_or in H1' as [? | ?];
-      eapply not_and_or in H2' as [? | H1''];
-      eapply not_and_or in H3' as [? | H2''];
-      try (eapply NNPP in H1'');
-      try (eapply NNPP in H2'');
-      eauto using UnsafeAccess
-    | assert (Hlen : ad' < length m) by eauto using access_length;
-      assert (~ SafeAccess m m[ad'] ad) by eauto using SafeAccess;
-      specialize (Hwtm _ Hlen) as [[? Htype'] ?]; eauto using UnsafeAccess
-    ];
-  intros F; destruct F; eauto using SafeAccess.
-Qed.
+SafeAccess m t ad ->
+t --> t'
+m[ad] = m'[ad]
 
-Theorem access_to_sacc : forall Gamma m t ad T,
-  Gamma |-- t is T ->
-  well_typed_memory m ->
-  access m t ad ->
-  ~ UnsafeAccess m t ad ->
-  SafeAccess m t ad.
-Proof.
-  intros * ? Hwtm Hacc ?.
-  generalize dependent Gamma. generalize dependent T.
-  induction Hacc; intros; inversion_type; eauto using SafeAccess;
-  unshelve solve 
-    [ exfalso; eauto using UnsafeAccess
-    | assert (~ UnsafeAccess m t ad) by shelve; eauto using SafeAccess
-    | assert (~ UnsafeAccess m t1 ad) by shelve;
-      assert (~ UnsafeAccess m t2 ad) by shelve;
-      eauto using SafeAccess
-    | assert (Hlen : ad' < length m) by eauto using access_length;
-      assert (~ UnsafeAccess m m[ad'] ad) by eauto using UnsafeAccess;
-      specialize (Hwtm _ Hlen) as [[? Htype'] ?]; eauto using SafeAccess
-    ];
-  intros F; destruct F; eauto using UnsafeAccess.
-Qed.
+m[ad] <> m'[ad]
+t --> t'
+UnsafeAccess m t ad
 
-Corollary sacc_uacc_dec : forall Gamma m t ad T,
-  well_typed_memory m ->
-  Gamma |-- t is T ->
-  access m t ad ->
-  (SafeAccess m t ad \/ UnsafeAccess m t ad).
-Proof.
-  intros. 
-  assert (decidable (UnsafeAccess m t ad)) as [? | ?] (* TODO *)
-      by eauto using classic_decidable.
-  - right. assumption.
-  - left. eauto using access_to_sacc.
-Qed.
-
+*)
